rowwise flatten (more fleshed-out) and proof outline

src/Experiments/SimplyTypedArithmetic.v
@@ -810,46 +810,6 @@ Module Columns.
           reflexivity. } }
     Qed.
 
-    Section Rows.
-
-      Let fw := (fun i => weight (S i) / weight i).
-
-      Fixpoint finish_row (idx: nat) (carry:Z) (inp: list (list Z)) : list (list Z) * Z :=
-        match inp with
-        | nil => (nil, carry)
-        | col :: inp' =>
-          match col with
-          | nil => ([carry] :: inp', 0) 
-          | x :: nil =>
-            let sum_carry := Z.add_with_get_carry_full (fw idx) carry x 0 in
-            let rec := finish_row (S idx) (snd sum_carry) inp' in
-            ([(fst sum_carry)] :: fst rec, snd rec)
-          | x :: y :: tl =>
-            let sum_carry := Z.add_with_get_carry_full (fw idx) carry x y in
-            let rec := finish_row (S idx) (snd sum_carry) inp' in
-            (((fst sum_carry) :: tl) :: fst rec, snd rec)
-          end
-        end.
-
-      Fixpoint flatten_rowwise' (start_value : Z) (start_col : list Z) (other_cols : list (list Z)) : list Z * Z :=
-        match start_col with
-        | nil => (start_value :: map sum other_cols, 0)
-        | x :: tl =>
-          let sum_carry := Z.add_get_carry_full (fw 0%nat) start_value x in
-          let other_cols'_carry := finish_row 1%nat (snd sum_carry) other_cols in
-          let rec := flatten_rowwise' (fst sum_carry) tl (fst other_cols'_carry) in
-          (fst rec, snd rec + snd other_cols'_carry)
-        end.
-
-      Definition flatten_rowwise (inp : list (list Z)) : list Z * Z :=
-        match inp with
-        | (x :: tl) :: other_cols =>
-          flatten_rowwise' x tl other_cols
-        | _ => (map sum inp, 0)
-        end.
-
-    End Rows.
-
     Section mul.
       Definition mul s n m (p q : list Z) : list Z :=
         let p_a := Positional.to_associational weight n p in
@@ -953,6 +913,169 @@ Module Columns.
 
   End mul_converted.
 End Columns.
+
+Module Rows.
+  Section Rows.
+    Context (weight : nat->Z)
+            {weight_0 : weight 0%nat = 1}
+            {weight_nonzero : forall i, weight i <> 0}
+            {weight_positive : forall i, weight i > 0}
+            {weight_multiples : forall i, weight (S i) mod weight i = 0}
+            {weight_divides : forall i : nat, weight (S i) / weight i > 0}.
+
+    Local Notation rows := (list (list Z)) (only parsing).
+    Local Notation cols := (list (list Z)) (only parsing).
+    Hint Rewrite Positional.eval_nil : push_eval.
+    Hint Resolve in_eq in_cons.
+
+    Definition eval n (inp : rows) :=
+      sum (map (Positional.eval weight n) inp).
+    Lemma eval_nil n : eval n nil = 0.
+    Proof. cbv [eval]. rewrite map_nil, sum_nil; reflexivity. Qed.
+    Hint Rewrite eval_nil : push_eval.
+    Lemma eval_cons n r inp : eval n (r :: inp) = Positional.eval weight n r + eval n inp.
+    Proof. cbv [eval]. rewrite map_cons, sum_cons; reflexivity. Qed.
+    Hint Rewrite eval_cons : push_eval.
+
+    Definition extract_row (inp : cols) : cols * list Z :=
+      fold_right (fun col state =>
+                    (tl col :: fst state, hd 0 col :: snd state)
+                 ) (nil, nil) inp.
+
+    Definition from_columns n (inp : cols) : rows :=
+      snd
+        (fold_right (fun _ (state : cols * rows) =>
+                       let cols'_row := extract_row (fst state) in
+                       (fst cols'_row, snd state ++ [snd cols'_row])
+                    ) (inp, nil) (seq 0 n)).
+
+    Lemma eval_from_columns (inp : cols) :
+      forall n m, length inp = n ->
+                (m = fold_right Nat.max 0%nat (map (@length Z) inp))%nat ->
+                eval n (from_columns m inp) = Columns.eval weight n inp.
+    Proof.
+      cbv [eval Columns.eval from_columns].
+      induction inp; intros; distr_length.
+      { subst n. subst m. reflexivity. }
+   Admitted.
+
+    Local Notation fw := (fun i => weight (S i) / weight i) (only parsing).
+
+    Definition sum_rows (row1 row2 : list Z) : list Z * Z :=
+      fold_left (fun (state : list Z * Z) next =>
+                    let i := length (fst state) in (* length of output accumulator tells us the index of [next] *)
+                    let sum_carry := Z.add_with_get_carry_full (fw i) (snd state) (fst next) (snd next) in
+                    (fst state ++ [fst sum_carry], snd sum_carry)) (combine row1 row2) (nil,0).
+
+    Definition flatten' (start_state : list Z * Z) (inp : rows) : list Z * Z :=
+      fold_right (fun next_row (state : list Z * Z)=>
+                    let out_carry := sum_rows next_row (fst state) in
+                    (fst out_carry, snd state + snd out_carry)) start_state inp.
+
+    (* For correctness if there is only one row, we add a row of
+    zeroes with the same length so that the add loop still happens. *)
+    Definition flatten (inp : rows) : list Z * Z :=
+      let first_row := hd nil inp in
+      flatten' (first_row, 0) (hd (Positional.zeros (length first_row)) (tl inp) :: tl (tl inp)).
+
+    Lemma sum_rows_mod row1 row2 n:
+      length row1 = n -> length row2 = n ->
+      Positional.eval weight n (fst (sum_rows row1 row2))
+      = (Positional.eval weight n row1 + Positional.eval weight n row2) mod (weight n).
+    Admitted.
+
+    Lemma sum_rows_div row1 row2 n:
+      length row1 = n -> length row2 = n ->
+      snd (sum_rows row1 row2)
+      = (Positional.eval weight n row1 + Positional.eval weight n row2) / (weight n).
+    Admitted.
+
+    Hint Rewrite sum_rows_mod using (auto; solve [distr_length; auto]) : push_eval.
+
+    Lemma sum_rows_partitions row1 row2 n i:
+      length row1 = n -> length row2 = n -> (i < n)%nat ->
+      nth_default 0 (fst (sum_rows row1 row2)) i
+      = ((Positional.eval weight n row1 + Positional.eval weight n row2) / weight i) mod (fw i).
+    Admitted.
+
+    Lemma length_sum_rows row1 row2 n :
+      length row1 = n -> length row2 = n ->
+      length (fst (sum_rows row1 row2)) = n.
+    Admitted.
+
+
+    (* TODO: move to ListUtil *)
+    (* connect state to remaining input *)
+    Lemma fold_right_invariant_strong {A B} (P: list B -> A -> Type) (f: B -> A -> A):
+      forall bs a0
+      (Pnil : P nil a0)
+      (IHfold:
+         forall bs' b a',
+           In b bs ->
+           a' = fold_right f a0 bs' ->
+          P bs' a' ->
+          P (b :: bs') (f b a')),
+      P bs (fold_right f a0 bs).
+    Proof. induction bs; intros; rewrite ?fold_right_cons; auto using in_eq,in_cons. Qed.
+
+    Lemma flatten'_div_mod n start_state inp:
+      length (fst start_state) = n ->
+      (forall row, In row inp -> length row = n) ->
+      length (fst (flatten' start_state inp)) = n
+        /\ (inp <> nil ->
+            Positional.eval weight n (fst (flatten' start_state inp)) = (Positional.eval weight n (fst start_state) + eval n inp) mod (weight n)
+            /\ snd (flatten' start_state inp) = snd start_state + (Positional.eval weight n (fst start_state) + eval n inp) / weight n).
+    Proof.
+      intro.
+      cbv [flatten'].
+      apply fold_right_invariant_strong with (bs:=inp); intros; [ tauto | destruct (dec (bs' = nil)) ];
+      repeat match goal with
+             | _ => subst a'
+             | _ => subst bs'
+             | _ => rewrite sum_rows_div with (n:=n) by auto
+             | _ => rewrite @fold_right_nil in *
+             | _ => progress autorewrite with cancel_pair push_eval in *
+             | H : _ -> _ /\ _ |- _ =>
+               let X := fresh in let Y := fresh in
+               destruct H as [X Y]; [ solve [auto using in_cons] | rewrite ?X, ?Y ]
+             | _ => split
+             | _ => progress autorewrite with pull_Zmod zsimplify_fast
+             | _ => solve [ auto using length_sum_rows ]
+             | _ => solve [ ring_simplify; repeat (f_equal; try ring) ]
+             end.
+      apply Z.mul_cancel_l with (p:=weight n); [ apply weight_nonzero |].
+      autorewrite with push_Zmul.
+      rewrite !Z.mul_div_eq_full by apply weight_nonzero.
+      autorewrite with pull_Zmod.
+      ring_simplify_subterms. ring_simplify.
+      repeat (f_equal; try ring).
+    Qed.
+
+    Hint Rewrite (@Positional.length_zeros weight) : distr_length.
+    Hint Rewrite (@Positional.eval_zeros weight) using auto : push_eval.
+
+    Lemma flatten_div_mod inp n :
+      (forall row, In row inp -> length row = n) ->
+      Positional.eval weight n (fst (flatten inp)) = (eval n inp) mod (weight n)
+      /\ snd (flatten inp) = (eval n inp) / weight n.
+    Proof.
+      intros; cbv [flatten].
+      destruct inp; [|destruct inp]; cbn [hd tl].
+      { cbn. autorewrite with push_eval. tauto. }
+      { cbn.
+        match goal with H : forall r, In r [?x] -> _ |- _ =>
+                        specialize (H x ltac:(auto)); rewrite H
+        end.
+        rewrite sum_rows_div with (n:=n) by distr_length.
+        autorewrite with push_eval.
+        split; f_equal; ring. }
+      { autorewrite with push_eval.
+        apply flatten'_div_mod; auto.
+        congruence. }
+      Qed.
+
+  End Rows.
+End Rows.
 
 Module Compilers.
   Module type.
